spsc-queue consume implementation (currently inconclusive)

concurrency/spsc-queue/QueueImpl.i.dfy
@@ -1,44 +1,224 @@
 include "../../lib/Lang/NativeTypes.s.dfy"
+include "../../lib/Base/LinearOption.i.dfy"
+include "../scache/GlinearOption.i.dfy"
 include "../framework/PCM.s.dfy"
 include "../framework/Ptrs.s.dfy"
 include "../framework/Atomic.s.dfy"
 include "../framework/MultiRw.i.dfy"
 include "QueueMultiRw.i.dfy"
 
-module QueueImpl {
+module QueueImpl(item: ItemModule) {
+  import opened Options
+  import opened LinearOption
+  import opened GlinearOption
   import opened GhostLoc
-  import opened Ptrs
+  import Ptrs
   import opened NativeTypes
   import opened Atomics
+  import opened QueueMultiRw = QueueMultiRw(item)
   import Tokens = MultiRwTokens(QueueMultiRw)
 
-  type Item(!new)
+  linear datatype ConsumerToken = ConsumerToken(glinear token: Tokens.Token, tail: uint32)
+  {
+    predicate Valid(loc: Loc) {
+      && this.token.loc == loc
 
-  linear datatype ConsumerToken = ConsumerToken(glinear token: Token, tail: uint32)
+      && this.token.val == M(None, None, map[], ProducerUnknown, ConsumerIdle(this.tail as nat))
+    }
+  }
+
+  linear datatype ProducerToken = ProducerToken(glinear token: Tokens.Token, head: uint32)
+  {
+    predicate Valid(loc: Loc) {
+      && this.token.loc == loc
+
+      && this.token.val == M(None, None, map[], ProducerIdle(this.head as nat), ConsumerUnknown)
+    }
+  }
 
   datatype Queue = Queue(
-    cells: seq<Ptr>,
-    head: Atomic<uint32, Token>,
-    tail: Atomic<uint32, Token>,
+    cells: seq<Ptrs.Ptr>,
+    head: Atomic<uint32, Tokens.Token>,
+    tail: Atomic<uint32, Tokens.Token>,
 
-    ghost cellToken: GhostAtomic<Token>,
+    ghost cellToken: GhostAtomic<Tokens.Token>,
     ghost loc: Loc
   ) {
 
-    method consume(linear consumerToken: ConsumerToken) returns (
-      linear consumerToken': ConsumerToken, linear item: Item)
+    predicate HeadInv(head_v: uint32, t: Tokens.Token, loc: Loc)
     {
-      atomic_block var ret_value := execute_atomic_load(this.head) {
+      && t.loc == loc
+      && t.val == M(Some(head_v as nat), None, map[], ProducerUnknown, ConsumerUnknown)
+    }
+
+    predicate TailInv(tail_v: uint32, t: Tokens.Token, loc: Loc)
+    {
+      && t.loc == loc
+      && t.val == M(None, Some(tail_v as nat), map[], ProducerUnknown, ConsumerUnknown)
+    }
+
+    predicate CellInv(t: Tokens.Token, loc: Loc)
+    requires |this.cells| == size()
+    {
+      && t.loc == loc
+      && exists cells_v :: (
+        && t.val == M(None, None, cells_v, ProducerUnknown, ConsumerUnknown)
+        && (forall i: nat | i < size() :: 
+          && i in cells_v.Keys
+          && ((cells_v[i].Full? || cells_v[i].Empty?) ==> cells_v[i].v.ptr == this.cells[i])
+          && (cells_v[i].Full? ==> cells_v[i].v.PointsToLinear?)
+          && (cells_v[i].Empty? ==> cells_v[i].v.PointsToEmpty?)
+        )
+      )
+    }
+
+    predicate Inv()
+    {
+      && this.loc.ExtLoc?
+      && this.loc.base_loc == Tokens.Wrap.singleton_loc()
+
+      && |this.cells| == size()
+
+      && this.head.namespace() == 1
+      && this.tail.namespace() == 2
+      && this.cellToken.namespace() == 3
+
+      && (forall v, g :: atomic_inv(this.head, v, g) <==> HeadInv(v, g, this.loc))
+      && (forall v, g :: atomic_inv(this.tail, v, g) <==> TailInv(v, g, this.loc))
+      && (forall v: (), g :: atomic_inv(this.cellToken, v, g) <==> CellInv(g, this.loc))
+    }
+
+    method consume(linear inout consumerToken: ConsumerToken)
+    returns (linear item: lOption<item.Item>)
+    requires this.Inv()
+    requires old_consumerToken.Valid(this.loc)
+    ensures consumerToken.Valid(this.loc)
+    {
+      linear var ConsumerToken(consumer_g, tail) := consumerToken;
+
+      glinear var pointsToCell;
+
+      atomic_block var head_value := execute_atomic_load(this.head) {
         ghost_acquire head_g;
         atomic_block var _ := execute_atomic_noop(this.cellToken) {
           ghost_acquire cellToken_g;
+
+          assert head_g.loc == cellToken_g.loc == consumer_g.loc;
+          assert head_g.val == M(Some(head_value as nat), None, map[], ProducerUnknown, ConsumerUnknown);
+          assert consumer_g.val == M(None, None, map[], ProducerUnknown, ConsumerIdle(tail as nat));
+
+          ghost var rest := Tokens.obtain_invariant_3(
+            inout consumer_g, inout head_g, inout cellToken_g);
+
+          ghost var m := dot(dot(consumer_g.val, head_g.val), cellToken_g.val);
+          assert MInv(dot(m, rest));
+
+          if head_value != tail {
+            assert dot(m, rest).cells[tail as nat].Full?;
+            assert cellToken_g.val.cells[tail as nat].Full?;
+
+            ghost var m' := m.(
+              consumer := ConsumerInProgress(tail as nat),
+              cells := m.cells[tail as nat := Consuming]);
+
+            ghost var consumer_g_val' := M(None, None, map[], ProducerUnknown, ConsumerInProgress(tail as nat));
+            ghost var cellToken_g_val' := cellToken_g.val.(cells := cellToken_g.val.cells[tail as nat := Consuming]);
+
+            assert m' == dot(dot(consumer_g_val', head_g.val), cellToken_g_val');
+
+            ghost var expected_v := cellToken_g.val.cells[tail as nat].v;
+            assert consumer_begin(m, m', expected_v);
+
+            consumer_begin_is_withdraw(m, m', expected_v);
+
+            assert withdraw(m, m', tail as nat, expected_v);
+
+            glinear var pointsToCell_v;
+            consumer_g, head_g, cellToken_g, pointsToCell_v :=
+              Tokens.withdraw_3_3(
+                consumer_g,
+                head_g,
+                cellToken_g, 
+
+                consumer_g_val',
+                head_g.val,
+                cellToken_g_val',
+
+                tail as nat,
+                expected_v);
+
+            pointsToCell := glSome(pointsToCell_v);
+          } else {
+            pointsToCell := glNone;
+          }
 
           ghost_release cellToken_g;
         }
         ghost_release head_g;
       }
+
+      if head_value != tail {
+        linear var item_v := this.cells[tail].read_linear(inout pointsToCell.value);
+        item := lSome(item_v);
+
+        var newTail := tail + 1;
+
+        atomic_block var _ := execute_atomic_store(this.tail, newTail) {
+          ghost_acquire tail_g;
+
+          atomic_block var _ := execute_atomic_noop(this.cellToken) {
+            ghost_acquire cellToken_g;
+
+            ghost var m := dot(dot(consumer_g.val, tail_g.val), cellToken_g.val);
+
+            ghost var rest := Tokens.obtain_invariant_3(
+              inout consumer_g, inout tail_g, inout cellToken_g);
+            
+            assert dot(m, rest).cells[tail as nat].Consuming?;
+            assert cellToken_g.val.cells[tail as nat].Consuming?;
+
+            glinear var depositing_v := GlinearOption.unwrap_value(pointsToCell);
+
+            ghost var m' := m.(
+              consumer := ConsumerIdle(newTail as nat),
+              tail := Some(newTail as nat),
+              cells := m.cells[tail as nat := Empty(depositing_v)]);
+
+            ghost var consumer_g_val' := consumer_g.val.(consumer := ConsumerIdle(newTail as nat));
+            ghost var tail_g_val' := tail_g.val.(tail := Some(newTail as nat));
+            ghost var cellToken_g_val' := cellToken_g.val.(cells := cellToken_g.val.cells[tail as nat := Empty(depositing_v)]);
+
+            assert m' == dot(dot(consumer_g_val', tail_g_val'), cellToken_g_val');
+
+            consumer_end_is_deposit(m, m', depositing_v);
+
+            consumer_g, tail_g, cellToken_g :=
+              Tokens.deposit_3_3(
+                consumer_g,
+                tail_g,
+                cellToken_g, 
+
+                tail as nat,
+                depositing_v,
+
+                consumer_g_val',
+                tail_g_val',
+                cellToken_g_val');
+
+            ghost_release cellToken_g;
+          }
+
+          ghost_release tail_g;
+        }
+
+      } else {
+        item := lNone;
+        GlinearOption.dispose_glnone(pointsToCell);
+      }
+
+      consumerToken := ConsumerToken(consumer_g, tail);
+      assert consumerToken.Valid(this.loc);
     }
 
   }
-  
 }
