concurrency/framework/MultiRw.i.dfy
@@ -211,11 +211,16 @@ module MultiRwTokens(rw: MultiRw) {
   ensures retrieved_value == expected_retrieved_value
 
   glinear method obtain_invariant_3(
-      glinear token1: Token,
-      glinear token2: Token,
-      glinear token3: Token)
+      glinear inout token1: Token,
+      glinear inout token2: Token,
+      glinear inout token3: Token)
   returns (ghost rest: rw.M)
-  requires token1.loc == token2.loc == token3.loc
+  requires old_token1.loc == old_token2.loc == old_token3.loc
+  ensures (
+    && old_token1 == token1
+    && old_token2 == token2
+    && old_token3 == token3
+  )
   ensures rw.Inv(rw.dot(rw.dot(rw.dot(token1.val, token2.val), token3.val), rest))
 
   // TODO borrow method
